\documentclass{article}
\pagenumbering{gobble}
\usepackage{amsfonts}
\usepackage{amsmath}

\begin{document}
If the vector $(2,6,1,-3)$ is a linear combination of the other vectors, the following equation should be solvable for constants $c_{1},c_{2},c_{3}\in \mathbb{R}$.

\[\begin{bmatrix} 2 \\ 6 \\ 1 \\ -3 \end{bmatrix} = c_{1}\vec{u} + c_{2}\vec{v} + c_{3}\vec{w}\]
\[\begin{bmatrix} 2 \\ 6 \\ 1 \\ -3 \end{bmatrix} = c_{1}\begin{bmatrix} 1 \\ 3 \\ 3 \\ 0 \end{bmatrix} + c_{2} \begin{bmatrix} 0 \\ 0 \\ 0 \\ 1 \end{bmatrix} + c_{3}\begin{bmatrix}0 \\ 0 \\ -5 \\ 0 \end{bmatrix}\]

This is equivalant to the following set of equations.
\[1c_{1}+0c_{2}+0c_{3}=2\]
\[3c_{1}+0c_{2}+0c_{3}=6\]
\[3c_{1}+0c_{2}+(-5)c_{3}=1\]
\[0c_{1}+1c_{2}+0c_{3}=-3\]
We can now solve for $c_{2}$
\[c_{2}=-3\]
Then for $c_{1}$
\[3c_{1}=6\]
\[c_{1}=2\]
Finally, for $c_{3}$
\[3c_{1}-5c_{3}=1\]
\[3(2)-5c_{3}=1\]
\[-5c_{3}=-5\]
\[c_{3}=1\]
Then we must verify that the values still work with the first equation.
\[1(2)+0(1)+0(-3)=2\]
\[2 = 2\]
Therefore, $(2.6.1.-3)$ is a linear combination of $\vec{v}, \vec{u}, \vec{w}$.
\end{document}
