\documentclass{article}
\pagenumbering{gobble}
\usepackage{amsfonts}
\usepackage{cancel}

\begin{document}
We can use the alternate form of $||\vec{v}||$ as $\sqrt{\vec{v}\cdot\vec{v}}$ to rewrite and re-arrange the initial equation.

\[||\vec{u}+\vec{v}||^{2}-||\vec{u}-\vec{v}||^{2}=\sqrt{(\vec{u}+\vec{v})\cdot(\vec{u}+\vec{v})}^{2}-\sqrt{(\vec{u}-\vec{v})\cdot(\vec{u}+\vec{v})}^{2}\]
\[= (\vec{u}+\vec{v})\cdot \vec{u} + (\vec{u}+\vec{v})\cdot \vec{v} - (\vec{u}-\vec{v}) \cdot \vec{u} - (\vec{u} - \vec{v}) \cdot (-\vec{v})\]
\[= \cancel{\vec{u}\cdot\vec{u}} + \vec{u}\cdot\vec{v} + \vec{u}\cdot\vec{v} +\cancel{\vec{v}\cdot\vec{v}} - \cancel{\vec{u}\cdot \vec{u}} + \vec{u} \cdot \vec{v} + \vec{u} \cdot \vec{v} - \cancel{\vec{v}\cdot \vec{v}}\]
\[=4\vec{u}\cdot\vec{v}\]
Therefore the preposition holds. From here we can prove the second part of the question using $\vec{u}\cdot\vec{v} = 0$ when $\vec{v}$ and $\vec{u}$ are orthogonal. We start by proving that $\vec{u}\cdot\vec{v}=0\Rightarrow||\vec{u}+\vec{v}|| = ||\vec{u}-\vec{v}||$.
\[4\vec{u}\cdot\vec{v} = ||\vec{u} + \vec{v}||^{2} - ||\vec{u} - \vec{v}||^{2}\]
\[4(0) = ||\vec{u} + \vec{v}||^{2} - ||\vec{u} - \vec{v}||^{2}\]
\[0  + ||\vec{u} - \vec{v}||^{2}= ||\vec{u} + \vec{v}||^{2}\]
\[||\vec{u} - \vec{v}||= ||\vec{u} + \vec{v}||\]
We then prove that $\vec{u}\cdot\vec{v}=0\Leftarrow||\vec{u}+\vec{v}|| = ||\vec{u}-\vec{v}||$. To do this we must first rearrange the length equation we initially proved.
\[4\vec{u}\cdot\vec{v} = ||\vec{u}+\vec{v}||^{2}-||\vec{u}-\vec{v}||^{2}\]
\[||\vec{u}+\vec{v}||^{2} = 4\vec{u}\cdot\vec{v} + ||\vec{u}-\vec{v}||^{2}\]
We can then substitute it into our initial premise after squaring both sides, and rearange.
\[||\vec{u}-\vec{v}||^{2}=||\vec{u}+\vec{v}||^{2}\]
\[||\vec{u}-\vec{v}||^{2}=4\vec{u}\cdot\vec{v}+||\vec{u}-\vec{v}||^{2}\]
\[0=4\vec{u}\cdot\vec{v}\]
\[0=\vec{u}\cdot\vec{v}\]
\end{document}
